---
layout: page
title: "Part 6: Power Series"
---

---

\\(
  \newcommand{\\<}{\langle}
  \newcommand{\\>}{\rangle}
\\) <!-- TODO make angle brackets parentheses -->



---

## 6.2 Taylor and Maclaurin Series

- University Calculus: Early Transcendentals (3rd Ed)
    - 9.8

### 6.2.1 Power Series from Functions

<iframe width="560" height="315" src="https://www.youtube.com/embed/7zjUV_jDrL8" frameborder="0" allowfullscreen></iframe>

- Let \\(f(x)\\) have derivatives of all orders nearby \\(a\\). Then the
  Taylor series generated by \\(f\\) at \\(a\\) is given by
  \\(\sum_{k=0}^\infty\frac{f^{(k)}(a)}{k!}(x-a)^k\\),
  where \\(f^{(k)}(a)\\) is the \\(k^{th}\\) derivative of \\(f\\) at \\(a\\).
- A Maclaurin series is a Taylor series where \\(a=0\\).
- A Taylor/Maclaurin series is said to converge to its generating function if
  it is equal to it for all members of its domain.
- **Example** Let \\(f(x)=\frac{1}{1+x}\\) with the domain \\(-1<x<1\\),
  and guess a formula for
  \\(f^{(k)}(0)\\) by computing its first few terms. Then show that
  the Maclaurin series generated by \\(f\\) converges to \\(f\\).
- **Example** Let \\(g(x)=\frac{2}{x}\\) with the domain \\(0<x<4\\),
  and guess a formula for
  \\(g^{(k)}(2)\\) by computing its first few terms. Then show that
  the Taylor series generated by \\(g\\) at \\(2\\) converges to \\(g\\).
- It can be shown that \\(f\\) defined by \\(f(0)=0\\) and
  \\(f(x)=e^{-1/x^2}\\) otherwise
  satisfies \\(f^{(k)}(0)=0\\), giving an example
  of a function which doesn't converge to its Taylor series.

### 6.2.2 Maclaurin Series for \\(e^x\\), \\(\\sin x\\), \\(\\cos x\\)

<iframe width="560" height="315" src="https://www.youtube.com/embed/D8g7uVFifTg" frameborder="0" allowfullscreen></iframe>

- The following Maclaurin Series can be shown to converge to their
  generating functions:
    - \\(e^x=\sum_{k=0}^\infty\frac{x^k}{k!}
      = 1+x+\frac{x^2}{2}+\frac{x^3}{6}+\dots\\)
    - \\(\cos x = \sum_{k=0}^\infty(-1)^k\frac{x^{2k}}{(2k)!}
      = 1-\frac{x^2}{2}+\frac{x^4}{24}-\frac{x^6}{720}+\dots\\)
    - \\(\sin x = \sum_{k=0}^\infty(-1)^k\frac{x^{2k+1}}{(2k+1)!}
      = x-\frac{x^3}{6}+\frac{x^5}{120}-\frac{x^7}{5040}+\dots\\)
- **Example** Show how to generate the Maclaurin series for \\(e^x\\).
- **Example** Show how to generate the Maclaurin series for \\(\sin x\\).

### 6.2.3 Composition, Differentiation, and Integration of Power Series

<iframe width="560" height="315" src="https://www.youtube.com/embed/u6HOtdNxp8o" frameborder="0" allowfullscreen></iframe>

- Power series may be manipulated by the multiplication and composition
  of continuous functions.
- **Example** Find a power series converging to \\(x\cos(-x^2)\\).
- Power series may be differentiated and integrated term-by-term.
  <!-- TODO note that doing these operations to
  Taylor series results in a Taylor series -->
- **Example** Find a power series converging to \\(\frac{1}{x^2-2x+1}\\)
  for \\(-1<x<1\\).

<iframe width="560" height="315" src="https://www.youtube.com/embed/BwoikeDgrOQ" frameborder="0" allowfullscreen></iframe>

- **Example** Find a power series converging to \\(\tan^{\leftarrow}(x)\\)
  for \\(-1<x<1\\).

### Exercises for 6.2

1.  Let \\(f(x)=\frac{1}{1-x}\\) with the domain \\(-1<x<1\\),
    and guess a formula for
    \\(f^{(k)}(0)\\) by computing its first few terms. Then show that
    the Maclaurin series generated by \\(f\\) converges to \\(f\\).
1.  Let \\(g(x)=\frac{3}{x}\\) with the domain \\(0<x<6\\),
    and guess a formula for
    \\(g^{(k)}(3)\\) by computing its first few terms. Then show that
    the Taylor series generated by \\(g\\) at \\(3\\) converges to \\(g\\).
1.  Show how to generate the Maclaurin series
    \\(\sum_{k=0}^\infty(-1)^k\frac{x^{2k}}{(2k)!}\\) for \\(\cos x\\).
1.  Find the Maclaurin series for \\(\sinh x\\).
1.  Find a power series converging to \\(\frac{x^3}{e^{x^2}}\\).
1.  Find a power series converging to \\(\frac{1}{x^2+2x+1}\\)
    for \\(|x|<1\\). (Hint: begin with the power series for
    \\(\frac{1}{1+x}\\) and then differentiate term-by-term.)
1.  Find a power series converging to \\(\ln|x|\\)
    for \\(0<x<2\\). (Hint: begin with the power series for
    \\(\frac{1}{1+x}\\) and then integrate term-by-term.)
1.  (QUIZ) Generate the Maclaurin Series for \\(\cosh x\\).
    - \\(\sum_{k=0}^\infty(-1)^k\frac{x^{2k+1}}{(2k+1)!}\\)
    - \\(\sum_{k=0}^\infty\frac{x^{2k}}{(2k)!}\\)
    - \\(\sum_{k=0}^\infty\frac{x^k}{(k+1)!}\\)
1.  (QUIZ) Find a power series converging to \\(x\cos x\\).
    - \\(\sum_{k=0}^\infty(-1)^k\frac{x^{2k+1}}{(2k)!}\\)
    - \\(\sum_{k=0}^\infty(-1)^k\frac{x^{2k}}{(2k+2)!}\\)
    - \\(\sum_{k=0}^\infty\frac{x^{2k+2}}{(2k+1)!}\\)
1.  (QUIZ) Find a power series converging to \\(\frac{d}{dx}[\sin(x^2)]\\).
    - \\(\sum_{k=0}^\infty\frac{(-x^2)^{4k+3}}{(4k+2)(2k)!}\\)
    - \\(\sum_{k=0}^\infty\frac{(2k+1)x^{2k+2}}{(2k+1)!}\\)
    - \\(\sum_{k=0}^\infty(-1)^k\frac{(4k+2)x^{4k+1}}{(2k+1)!}\\)

[Solutions 1-4]({{site.baseurl}}public/solutions/6.2a.pdf)

[Solutions 5-10]({{site.baseurl}}public/solutions/6.2b.pdf)


---

## 6.3 Convergence of Taylor Series

- University Calculus: Early Transcendentals (3rd Ed)
    - 9.9

### 6.3.1 Taylor's Formula

<iframe width="560" height="315" src="https://www.youtube.com/embed/qmnRH1TgNZc" frameborder="0" allowfullscreen></iframe>

- Taylor's Formula guarantees that if \\(f\\) has derivatives of all orders
  on an open interval containing \\(a\\), then for every nonnegative integer
  \\(n\\) and \\(x\\) in that same interval,
  \\(f(x)=\left(\sum_{k=0}^n\frac{f^{(k)}(a)}{k!}(x-a)^k\right)+R_n(x)\\)
  where the error term is given by
  \\(R_n(x)=\frac{f^{(n+1)}(x_n)}{(n+1)!}(x-a)^{n+1}\\) for some number
  \\(x_n\\) between \\(a\\) and \\(x\\).
- **Example** Use the fact that \\(e<4\\) and Taylor's Formula to estimate
  the value of \\(\sqrt{e}\\) with an error no greater than \\(0.01\\).
- **Example** Use Taylor's Formula to estimate
  the value of \\(\sin(0.1)\\) with an error no greater than \\(0.0001\\).


### 6.3.2 Convergence of Taylor and Maclaurin Series

<iframe width="560" height="315" src="https://www.youtube.com/embed/9iBMea-InTQ" frameborder="0" allowfullscreen></iframe>

- A Taylor series converges to its generating function when
  \\(\lim_{n\to\infty}\|R_n(x)\|=0\\).
- **Example** Prove that \\(e^x=\sum_{k=0}^\infty\frac{x^k}{k!}\\).
- **Example** Prove that
  \\(\cos(x)=\sum_{k=0}^\infty(-1)^k\frac{x^{2k}}{(2k)!}\\).


### Exercises for 6.3

1.  Use the fact that \\(e<3\\) and
    Taylor's Formula to estimate the value of \\(e\\) with an error
    no greater than \\(0.001\\).
1.  Use Taylor's Formula to estimate the value of \\(\cos(0.1)\\) with an error
    no greater than \\(0.0001\\).
1.  Use Taylor's Formula to estimate the value of \\(\sin(1)\\) with an error
    no greater than \\(0.01\\).
1.  Prove that \\(\sin(x)=\sum_{k=0}^\infty(-1)^k\frac{x^{2k+1}}{(2k+1)!}\\).
1.  Use the fact that \\(\|\sinh(x_n)\|\leq\|\cosh(x_n)\|\leq\cosh(x)\\)
    for any \\(x_n\\) between \\(0\\) and \\(x\\) to
    prove that \\(\cosh(x)=\sum_{k=0}^\infty\frac{x^{2k}}{(2k)!}\\).
1.  Reprove \\(\cosh(x)=\sum_{k=0}^\infty\frac{x^{2k}}{(2k)!}\\) by using
    its definition \\(\cosh(x)=\frac{1}{2}(e^x+e^{-x})\\) along with
    the Maclaurin series for \\(e^x\\).
1.  (OPTIONAL) Prove that \\(\|\sinh(x_n)\|\leq\|\cosh(x_n)\|\leq\cosh(x)\\)
    for any \\(x_n\\) between \\(0\\) and \\(x\\).
1.  (QUIZ)
    Which of these Maclaurin Series is most appropriate for approximating
    \\(e^{-1/2}=\frac{1}{\sqrt e}\\)?
    - \\(\sum_{k=0}^\infty(-1)^k\frac{x^{2k+1}}{(2k+1)!}\\)
    - \\(\sum_{k=0}^\infty(-1)^k\frac{x^{2k}}{(2k)!}\\)
    - \\(\sum_{k=0}^\infty\frac{x^k}{k!}\\)
1.  (QUIZ)
    Find the error term \\(R_n(x)\\) from the Taylor Formula for \\(e^x\\),
    where \\(x_n\\) is between \\(0\\) and \\(x\\).
    - \\(R_n(x)=\frac{x^{n+1}}{n!}\\)
    - \\(R_n(x)=\frac{e^{x_n}}{(n+1)!}x^{n+1}\\)
    - \\(R_n(x)=\frac{1}{e^{x_n/2}(n+1)!}x^n\\)
1.  (QUIZ)
    Use Taylor's Formula to
    approximate \\(e^{-1/2}=\frac{1}{\sqrt e}\\) with an error no greater than
    \\(\frac{1}{1000}=0.001\\). (Hint: \\(-1/2\leq x_n\leq 0\\).)
    - \\(\frac{1}{\sqrt e}\approx 0.604\\)
    - \\(\frac{1}{\sqrt e}\approx 0.607\\)
    - \\(\frac{1}{\sqrt e}\approx 0.609\\)

[Solutions 1-7]({{site.baseurl}}public/solutions/6.3a.pdf)

[Solutions 8-10]({{site.baseurl}}public/solutions/6.3b.pdf)
