---
layout: page
title: Section 6.2 Calculus 2
header-img: "/assets/img/cal2-bg.png"
description: Taylor and Maclaurin Series
---

[Back to Table of Contents](../..)

---

## 6.2 Taylor and Maclaurin Series

### 6.2.1 Power Series from Functions

<iframe width="560" height="315" src="https://www.youtube.com/embed/7zjUV_jDrL8" frameborder="0" allowfullscreen></iframe>

- Let \\(f(x)\\) have derivatives of all orders nearby \\(a\\). Then the
  Taylor series generated by \\(f\\) at \\(a\\) is given by
  \\(\sum_{k=0}^\infty\frac{f^{(k)}(a)}{k!}(x-a)^k\\),
  where \\(f^{(k)}(a)\\) is the \\(k^{th}\\) derivative of \\(f\\) at \\(a\\).
- A Maclaurin series is a Taylor series where \\(a=0\\).
- A Taylor/Maclaurin series is said to converge to its generating function if
  it is equal to it for all members of its domain.
- **Example** Let \\(f(x)=\frac{1}{1+x}\\) with the domain \\(-1<x<1\\),
  and guess a formula for
  \\(f^{(k)}(0)\\) by computing its first few terms. Then show that
  the Maclaurin series generated by \\(f\\) converges to \\(f\\).
- **Example** Let \\(g(x)=\frac{2}{x}\\) with the domain \\(0<x<4\\),
  and guess a formula for
  \\(g^{(k)}(2)\\) by computing its first few terms. Then show that
  the Taylor series generated by \\(g\\) at \\(2\\) converges to \\(g\\).
- It can be shown that \\(f\\) defined by \\(f(0)=0\\) and
  \\(f(x)=e^{-1/x^2}\\) otherwise
  satisfies \\(f^{(k)}(0)=0\\), giving an example
  of a function which doesn't converge to its Taylor series.
- If a power series of the form
  \\(\sum_{k=0}^\infty\frac{f^{(k)}(a)}{k!}(x-a)^k\\) converges to
  \\(f(x)\\), then that power series is the Taylor series generated by
  \\(f(x)\\) at \\(a\\).

### 6.2.2 Maclaurin Series for \\(e^x\\), \\(\\sin x\\), \\(\\cos x\\)

<iframe width="560" height="315" src="https://www.youtube.com/embed/D8g7uVFifTg" frameborder="0" allowfullscreen></iframe>

- The following Maclaurin Series can be shown to converge to their
  generating functions:
    - \\(e^x=\sum_{k=0}^\infty\frac{x^k}{k!}
      = 1+x+\frac{x^2}{2}+\frac{x^3}{6}+\dots\\)
    - \\(\cos x = \sum_{k=0}^\infty(-1)^k\frac{x^{2k}}{(2k)!}
      = 1-\frac{x^2}{2}+\frac{x^4}{24}-\frac{x^6}{720}+\dots\\)
    - \\(\sin x = \sum_{k=0}^\infty(-1)^k\frac{x^{2k+1}}{(2k+1)!}
      = x-\frac{x^3}{6}+\frac{x^5}{120}-\frac{x^7}{5040}+\dots\\)
- **Example** Show how to generate the Maclaurin series for \\(e^x\\).
- **Example** Show how to generate the Maclaurin series for \\(\sin x\\).

---

### Review Exercises

1.  Let \\(f(x)=\frac{1}{1-x}\\) with the domain \\(-1<x<1\\),
    and guess a formula for
    \\(f^{(k)}(0)\\) by computing its first few terms. Then show that
    the Maclaurin series generated by \\(f\\) converges to \\(f\\).
1.  Let \\(g(x)=\frac{3}{x}\\) with the domain \\(0<x<6\\),
    and guess a formula for
    \\(g^{(k)}(3)\\) by computing its first few terms. Then show that
    the Taylor series generated by \\(g\\) at \\(3\\) converges to \\(g\\).
1.  Let \\(h(x)=\frac{1}{x^2+1}\\) with the domain \\(-1<x<1\\).
    It may be shown that the first few terms of
    \\(\\<h^{(k)}(0)\\>\_{k=0}^\infty\\)
    are \\(\\<1,0,-2,0,24,0,-720,\dots\\>\\). Show that
    the Maclaurin series generated by \\(h\\) converges to \\(h\\).
1.  Show how to generate the Maclaurin series
    \\(\sum_{k=0}^\infty(-1)^k\frac{x^{2k}}{(2k)!}\\) for \\(\cos x\\).
1.  Find the Maclaurin series for \\(\sinh x\\).
1.  Find the Maclaurin series for \\(\cosh x\\).
1.  Find the Maclaurin series for \\(e^{-x}\\).
1.  Find the Maclaurin series for \\(x^3+3x-7\\).

[Solutions](/resources/calculus2/solutions/6.2.pdf)

---

### Textbook References

- University Calculus: Early Transcendentals (3rd Ed)
    - 9.8
