---
layout: page
title: Section 6.4 Calculus 2
header-img: "/assets/img/cal2-bg.png"
description: Taylor's Formula
---

[Back to Table of Contents](../..)

---

## 6.4 Taylor's Formula

### 6.4.1 Taylor's Formula

<iframe width="560" height="315" src="https://www.youtube.com/embed/qmnRH1TgNZc" frameborder="0" allowfullscreen></iframe>

- Taylor's Formula guarantees that if \\(f\\) has derivatives of all orders
  on an open interval containing \\(a\\), then for every nonnegative integer
  \\(n\\) and \\(x\\) in that same interval,
  \\(f(x)=\left(\sum_{k=0}^n\frac{f^{(k)}(a)}{k!}(x-a)^k\right)+R_n(x)\\)
  where the error term is given by
  \\(R_n(x)=\frac{f^{(n+1)}(x_n)}{(n+1)!}(x-a)^{n+1}\\) for some number
  \\(x_n\\) between \\(a\\) and \\(x\\).
- **Example** Use the fact that \\(e<4\\) and Taylor's Formula to estimate
  the value of \\(\sqrt{e}\\) with an error no greater than \\(0.01\\).
- **Example** Use Taylor's Formula to estimate
  the value of \\(\sin(0.1)\\) with an error no greater than \\(0.0001\\).


### 6.4.2 Convergence of Taylor and Maclaurin Series

<iframe width="560" height="315" src="https://www.youtube.com/embed/9iBMea-InTQ" frameborder="0" allowfullscreen></iframe>

- A Taylor series converges to its generating function when
  \\(\lim_{n\to\infty}\|R_n(x)\|=0\\).
- **Example** Prove that \\(e^x=\sum_{k=0}^\infty\frac{x^k}{k!}\\).
- **Example** Prove that
  \\(\cos(x)=\sum_{k=0}^\infty(-1)^k\frac{x^{2k}}{(2k)!}\\).

---

### Review Exercises

1.  Use the fact that \\(e<3\\) and
    Taylor's Formula to estimate the value of \\(e\\) with an error
    no greater than \\(0.001\\).
1.  Use Taylor's Formula to estimate the value of \\(\cos(0.1)\\) with an error
    no greater than \\(0.0001\\).
1.  Use Taylor's Formula to estimate the value of \\(\sin(1)\\) with an error
    no greater than \\(0.01\\).
1.  Prove that \\(\sin(x)=\sum_{k=0}^\infty(-1)^k\frac{x^{2k+1}}{(2k+1)!}\\).
1.  Use the fact that \\(\|\sinh(x_n)\|\leq\|\cosh(x_n)\|\leq\cosh(x)\\)
    for any \\(x_n\\) between \\(0\\) and \\(x\\) to
    prove that \\(\cosh(x)=\sum_{k=0}^\infty\frac{x^{2k}}{(2k)!}\\).
1.  Reprove \\(\cosh(x)=\sum_{k=0}^\infty\frac{x^{2k}}{(2k)!}\\) by using
    its definition \\(\cosh(x)=\frac{1}{2}(e^x+e^{-x})\\) along with
    the Maclaurin series for \\(e^x\\).

[Solutions](/resources/calculus2/solutions/6.4.pdf)
